finished definitions of swap lemmas

GateHelpers.v
@@ -4,6 +4,7 @@ From Proof Require Import SwapHelpers.
 Definition abgate (U : Square 4) := U ⊗ I 2.
 Definition bcgate (U : Square 4) := I 2 ⊗ U.
 Definition acgate (U : Square 4) := swapbc × (abgate U) × swapbc.
+Definition ccu (U : Square 2) := control (control U).
 
 Lemma WF_abgate : forall (U : Square 4), WF_Matrix U -> WF_Matrix (abgate U).
 Proof.
@@ -30,6 +31,11 @@ apply WF_abgate. apply H.
 apply WF_swapbc.
 Qed.
 
+Lemma WF_ccu : forall (U : Square 2), WF_Matrix U -> WF_Matrix (ccu U).
+Proof.
+intros. apply WF_control. apply WF_control. apply H.
+Qed.
+
 Lemma abgate_unitary : forall (U : Square 4), WF_Unitary U -> WF_Unitary (abgate U).
 Proof.
 intros.
@@ -49,4 +55,10 @@ apply Mmult_unitary. apply Mmult_unitary.
 apply swapbc_unitary.
 apply abgate_unitary. apply H.
 apply swapbc_unitary.
+Qed.
+
+Lemma ccu_unitary : forall (U : Square 2), WF_Unitary U -> WF_Unitary (ccu U).
+Proof.
+intros.
+apply control_unitary. apply control_unitary. apply H.
 Qed.
